[Parikh] documentation for Eq_Sys.thy

Parikh/Eq_Sys.thy
@@ -1,121 +1,52 @@
+section \<open>Context free grammars and systems of equations\<close>
+
 theory Eq_Sys
   imports
     "Parikh_Img"
     "CFG.CFL"
 begin
 
-(* TODO: remove unnecessary definitions and rename *)
-
-text \<open>In his proof, Pilling uses the fact that each CFG has an associated system of equations such
-that the CFG is the system's minimal solution. In this file, we will introduce for a given CFG two
-equation systems - one which assumes that the alphabet is commutative, i.e. only considers
-the languages' parikh images, and one which does not make this assumption - and show that the CFG
-is indeed the minimal solution of both.\<close>
+text \<open>In this section, we will first introduce two types of systems of
+equations. Then we will show that to each CFG correspond two systems of equations - one for both of the types -
+and that the language defined by the CFG is a minimal solution of both systems.\<close>
 
 
-section \<open>systems of equations\<close>
+subsection \<open>Introduction of systems of equations\<close>
 
-text \<open>Given an system of equations
-\<open>X\<^sub>0 \<supseteq> r\<^sub>0, X\<^sub>1 \<supseteq> r\<^sub>1, X\<^sub>2 \<supseteq> r\<^sub>2, \<dots>\<close> or \<open>\<Psi> X\<^sub>0 \<supseteq> \<Psi> r\<^sub>0, \<Psi> X\<^sub>1 \<supseteq> \<Psi> r\<^sub>1, \<Psi> X\<^sub>2 \<supseteq> \<Psi> r\<^sub>2, \<dots>\<close>
-(depending on the context), we represent it as a list of of language functions where we identify
-each of the variables \<open>X\<^sub>0, X\<^sub>1, X\<^sub>2, \<dots>\<close>, by its integer, i.e. \<open>Var i\<close> denotes the variable \<open>X\<^sub>i\<close>.
-The \<open>i\<close>-th item of the list then represents the right-hand side \<open>r\<^sub>i\<close> of the \<open>i\<close>-th equation.\<close>
+text \<open>For the first type of systems, each equation is of the form
+\<^latex>\<open>$$X_i \supseteq r_i$$\<close>
+For the second type of systems, each equation is of the form
+\<^latex>\<open>$$\Psi \; X_i \supseteq \Psi \; r_i$$\<close>
+i.e. the Parikh image is applied on both sides of each equation.
+In both cases, we represent the whole system by a list of regular language expression where each of the variables
+\<open>X\<^sub>0, X\<^sub>1, \<dots>\<close> is identified by its integer, i.e. \<^term>\<open>Var i\<close> denotes the variable \<open>X\<^sub>i\<close>.
+The \<open>i\<close>-th item of the list then represents the right-hand side \<open>r\<^sub>i\<close> of the \<open>i\<close>-th equation:\<close>
 
 type_synonym 'a eq_sys = "'a rlexp list"
 
 
-subsection \<open>system of equations without Parikh images\<close>
-
-text \<open>Now we can define what it means for a valuation \<open>v\<close> to solve the classic system of equations,
-i.e. the one without Parikh images:\<close>
+text \<open>Now we can define what it means for a valuation \<open>v\<close> to solve a system of equations of the first type,
+i.e. a system without Parikh images. Afterwards we characterize minimal solutions of such a system.\<close>
 definition solves_ineq_sys :: "'a eq_sys \<Rightarrow> 'a valuation \<Rightarrow> bool" where
   "solves_ineq_sys sys v \<equiv> \<forall>i < length sys. eval (sys ! i) v \<subseteq> v i"
 
-(* solves equation with = *)
-definition solves_eq_sys :: "'a eq_sys \<Rightarrow> 'a valuation \<Rightarrow> bool" where
-  "solves_eq_sys sys v \<equiv> \<forall>i < length sys. eval (sys ! i) v = v i"
-
-text \<open>\<open>sol\<close> is a minimal solution iff it is a solution and there is no smaller solution:\<close>
 definition min_sol_ineq_sys :: "'a eq_sys \<Rightarrow> 'a valuation \<Rightarrow> bool" where
   "min_sol_ineq_sys sys sol \<equiv>
     solves_ineq_sys sys sol \<and> (\<forall>sol'. solves_ineq_sys sys sol' \<longrightarrow> (\<forall>x. sol x \<subseteq> sol' x))"
 
 
-subsection \<open>System of equations with Parikh images\<close>
-
-text \<open>Now we look at the system of equations where the Parikh image is applied on both sides of
-each equation. First, we introduce what it means for a valuation \<open>v\<close> to solve the \<open>x\<close>-th equation:\<close>
-(* solves equation with \<subseteq>, only caring about the Parikh image *)
+text \<open>The previous definitions can easily be extended to the second type of systems of equations where the Parikh image is applied on both sides of
+each equation:\<close>
 definition solves_ineq_comm :: "nat \<Rightarrow> 'a rlexp \<Rightarrow> 'a valuation \<Rightarrow> bool" where
   "solves_ineq_comm x eq v \<equiv> parikh_img (eval eq v) \<subseteq> parikh_img (v x)"
 
-text \<open>A valuation \<open>v\<close> solves the whole system iff it solves all equations:\<close>
-(* solves equation system with \<subseteq>, only caring about the Parikh image *)
 definition solves_ineq_sys_comm :: "'a eq_sys \<Rightarrow> 'a valuation \<Rightarrow> bool" where
   "solves_ineq_sys_comm sys v \<equiv> \<forall>i < length sys. solves_ineq_comm i (sys ! i) v"
 
-(* solves equation with =, only caring about the Parikh image*)
-definition solves_eq_comm :: "nat \<Rightarrow> 'a rlexp \<Rightarrow> 'a valuation \<Rightarrow> bool" where
-  "solves_eq_comm x eq v \<equiv> parikh_img (eval eq v) = parikh_img (v x)"
-
-(* solves equation system with =, only caring about the Parikh image *)
-definition solves_eq_sys_comm :: "'a eq_sys \<Rightarrow> 'a valuation \<Rightarrow> bool" where
-  "solves_eq_sys_comm sys v \<equiv> \<forall>i < length sys. solves_eq_comm i (sys ! i) v"
-
-text \<open>We introduce partial solutions, i.e. solutions which might depend on one or multiple variables.
-They are therefore not represented as valuations, but as language functions (TODO). \<open>sol\<close> is a partial
-solution of the \<open>x\<close>-th equation iff it solves the equation independent on the values of the other
-variables, i.e. independent on the valuation as long as the valuation and \<open>sol\<close> coincide.
-Note that \<open>sol\<close> might depend on the variable \<open>x\<close> (we will deal with this problem later)\<close>
-definition partial_sol_ineq :: "nat \<Rightarrow> 'a rlexp \<Rightarrow> 'a rlexp \<Rightarrow> bool" where
-  "partial_sol_ineq x eq sol \<equiv> \<forall>v. v x = eval sol v \<longrightarrow> solves_ineq_comm x eq v"
-
-text \<open>We generalize this to partial solutions of whole systems of equations:
-\<open>sols\<close> maps each variable \<open>i\<close> to a language function (TODO) representing the partial solution
-of the \<open>i\<close>-th equation (Note that \<open>sols\<close> is defined on all natural numbers, though).
-\<open>sols\<close> is a partial solution of the whole system iff all valuations coinciding with \<open>sols\<close> solve
-the system of equations:\<close>
-definition solution_ineq_sys :: "'a eq_sys \<Rightarrow> (nat \<Rightarrow> 'a rlexp) \<Rightarrow> bool" where
-  "solution_ineq_sys sys sols \<equiv> \<forall>v. (\<forall>x. v x = eval (sols x) v) \<longrightarrow> solves_ineq_sys_comm sys v"
-
-text \<open>Given a system of equations \<open>sys\<close>, \<open>sols\<close> is a minimal partial solution of the first \<open>n\<close>
-equations of the system iff the following conditions are satisfied:
-1. \<open>sols\<close> is a partial solution of the system's first \<open>n\<close> equations
-2. \<open>sols\<close> does not assign a proper partial solution to the remaining equations,
-   i.e. \<open>sols i = Var i\<close> for \<open>i \<ge> n\<close>
-3. No language function (TODO) in \<open>sols\<close> depends on variables smaller than \<open>n\<close>.
-   Furthermore, the partial solution of no equation depends on variables not occurring in the equation system
-4. There is no partial solution smaller than \<open>sols\<close> which solves all of the first \<open>n\<close> equations\<close>
-definition partial_min_sol_ineq_sys :: "nat \<Rightarrow> 'a eq_sys \<Rightarrow> (nat \<Rightarrow> 'a rlexp) \<Rightarrow> bool" where
-  "partial_min_sol_ineq_sys n sys sols \<equiv>
-    solution_ineq_sys (take n sys) sols \<and>
-    (\<forall>i \<ge> n. sols i = Var i) \<and>
-    (\<forall>i < n. \<forall>x \<in> vars (sols i). x \<ge> n \<and> x < length sys) \<and>
-    (\<forall>sols' v'. (\<forall>x. v' x = eval (sols' x) v')
-                  \<and> solves_ineq_sys_comm (take n sys) v'
-                  \<longrightarrow> (\<forall>i. parikh_img (eval (sols i) v') \<subseteq> parikh_img (v' i)))"
-
-
-text \<open>Given the \<open>x\<close>-th equation \<open>eq\<close>, \<open>sol\<close> is a minimal partial solution of this equation iff
-1. \<open>sol\<close> is a partial solution of \<open>eq\<close>,
-2. \<open>sol\<close> is a proper partial solution (i.e. it does not depend on \<open>x\<close>) and only depends on variables
-   occurring in the equation \<open>eq\<close> and
-3. no partial solution of the equation \<open>eq\<close> is smaller than \<open>sol\<close>\<close>
-definition partial_min_sol_one_ineq :: "nat \<Rightarrow> 'a rlexp \<Rightarrow> 'a rlexp \<Rightarrow> bool" where
-  "partial_min_sol_one_ineq x eq sol \<equiv>
-    partial_sol_ineq x eq sol \<and>
-    vars sol \<subseteq> vars eq - {x} \<and>
-    (\<forall>sol' v'. solves_ineq_comm x eq v' \<and> v' x = eval sol' v'
-               \<longrightarrow> parikh_img (eval sol v') \<subseteq> parikh_img (v' x))"
-
-
-text \<open>\<open>sol\<close> is a minimal solution of the system \<open>sys\<close> of equations iff it is a solution
-and there is no smaller solution:\<close>
 definition min_sol_ineq_sys_comm :: "'a eq_sys \<Rightarrow> 'a valuation \<Rightarrow> bool" where
   "min_sol_ineq_sys_comm sys sol \<equiv>
     solves_ineq_sys_comm sys sol \<and>
     (\<forall>sol'. solves_ineq_sys_comm sys sol' \<longrightarrow> (\<forall>x. parikh_img (sol x) \<subseteq> parikh_img (sol' x)))"
-
 
 text \<open>Substitution into each equation of a system:\<close>
 definition subst_sys :: "(nat \<Rightarrow> 'a rlexp) \<Rightarrow> 'a eq_sys \<Rightarrow> 'a eq_sys" where
@@ -127,7 +58,51 @@ lemma subst_sys_subst:
   unfolding subst_sys_def by (simp add: assms)
 
 
-text \<open>If the parikh image of two equations \<open>f\<close> and \<open>g\<close> is identical on all valuations, then their
+subsection \<open>Partial solutions of systems of equations\<close>
+
+text \<open>We introduce partial solutions, i.e. solutions which might depend on one or multiple variables.
+They are therefore not represented as valuations, but as regular language expressions. \<open>sol\<close> is a partial
+solution of the \<open>x\<close>-th equation if and only if it solves the equation independently on the values of the other
+variables:\<close>
+definition partial_sol_ineq :: "nat \<Rightarrow> 'a rlexp \<Rightarrow> 'a rlexp \<Rightarrow> bool" where
+  "partial_sol_ineq x eq sol \<equiv> \<forall>v. v x = eval sol v \<longrightarrow> solves_ineq_comm x eq v"
+
+text \<open>We generalize the previous definition to partial solutions of whole systems of equations:
+\<open>sols\<close> maps each variable \<open>i\<close> to a regular language expression representing the partial solution
+of the \<open>i\<close>-th equation. A partial solution of the whole system is then defined as follows:\<close>
+definition solution_ineq_sys :: "'a eq_sys \<Rightarrow> (nat \<Rightarrow> 'a rlexp) \<Rightarrow> bool" where
+  "solution_ineq_sys sys sols \<equiv> \<forall>v. (\<forall>x. v x = eval (sols x) v) \<longrightarrow> solves_ineq_sys_comm sys v"
+
+text \<open>Given the \<open>x\<close>-th equation \<open>eq\<close>, \<open>sol\<close> is a minimal partial solution of this equation if and only if
+\<^latex>\<open>\begin{enumerate}
+\item \textit{sol} is a partial solution of \textit{eq}
+\item \textit{sol} is a proper partial solution (i.e. it does not depend on \textit{x}) and only
+  depends on variables occurring in the equation \textit{eq}
+\item no partial solution of the equation \textit{eq} is smaller than \textit{sol}
+\end{enumerate}\<close>\<close>
+definition partial_min_sol_one_ineq :: "nat \<Rightarrow> 'a rlexp \<Rightarrow> 'a rlexp \<Rightarrow> bool" where
+  "partial_min_sol_one_ineq x eq sol \<equiv>
+    partial_sol_ineq x eq sol \<and>
+    vars sol \<subseteq> vars eq - {x} \<and>
+    (\<forall>sol' v'. solves_ineq_comm x eq v' \<and> v' x = eval sol' v'
+               \<longrightarrow> parikh_img (eval sol v') \<subseteq> parikh_img (v' x))"
+
+text \<open>Given a whole system of equations \<open>sys\<close>, we can generalize the previous definition such that
+\<open>sols\<close> is a minimal solution of the first \<open>n\<close> equations that might depend on the variables
+\<^latex>\<open>$X_n, X_{n+1}, \dots$\<close> Besides the three conditions described above,
+we introduce a forth condition: \<open>sols i = Var i\<close> for \<open>i \<ge> n\<close>, i.e. \<open>sols\<close> assigns only spurious solutions
+to the equations which are not yet solved:\<close>
+definition partial_min_sol_ineq_sys :: "nat \<Rightarrow> 'a eq_sys \<Rightarrow> (nat \<Rightarrow> 'a rlexp) \<Rightarrow> bool" where
+  "partial_min_sol_ineq_sys n sys sols \<equiv>
+    solution_ineq_sys (take n sys) sols \<and>
+    (\<forall>i \<ge> n. sols i = Var i) \<and>
+    (\<forall>i < n. \<forall>x \<in> vars (sols i). x \<ge> n \<and> x < length sys) \<and>
+    (\<forall>sols' v'. (\<forall>x. v' x = eval (sols' x) v')
+                  \<and> solves_ineq_sys_comm (take n sys) v'
+                  \<longrightarrow> (\<forall>i. parikh_img (eval (sols i) v') \<subseteq> parikh_img (v' i)))"
+
+
+text \<open>If the Parikh image of two equations \<open>f\<close> and \<open>g\<close> is identical on all valuations, then their
 minimal partial solution is identical, too:\<close>
 lemma same_min_sol_if_same_parikh_img:
   assumes same_parikh_img: "\<forall>v. parikh_img (eval f v) = parikh_img (eval g v)"
@@ -147,10 +122,12 @@ qed
 
 
 
-section \<open>CFG as minimal solution of equation system\<close>
+subsection \<open>CFLs as minimal solution of systems of equations\<close>
 
-text \<open>We show that each CFG induces a system of equations such that the CFG's language is the
-minimal solution of this system\<close>
+text \<open>We show that each CFG induces a system of equations of the first type, i.e. without Parikh images,
+such that the CFG's language is the minimal solution of the system. First, we describe how to derive
+the system of equations from a CFG. This requires us to fix some bijection between the variables in
+the system and the non-terminals occurring in the CFG:\<close>
 
 definition bij_Nt_Var :: "'n set \<Rightarrow> (nat \<Rightarrow> 'n) \<Rightarrow> ('n \<Rightarrow> nat) \<Rightarrow> bool" where
   "bij_Nt_Var A \<gamma> \<gamma>' \<equiv> bij_betw \<gamma> {..< card A} A \<and> bij_betw \<gamma>' A {..< card A}
@@ -169,34 +146,6 @@ proof -
 qed
 
 
-definition rlexp_sym :: "('n \<Rightarrow> nat) \<Rightarrow> ('n, 't) sym \<Rightarrow> 't rlexp" where
-  "rlexp_sym \<gamma>' s = (case s of Tm a \<Rightarrow> Const {[a]} | Nt A \<Rightarrow> Var (\<gamma>' A))"
-
-definition rlexp_concats :: "'a rlexp list \<Rightarrow> 'a rlexp" where
-  "rlexp_concats fs = foldr Concat fs (Const {[]})"
-
-definition rlexp_syms :: "('n \<Rightarrow> nat) \<Rightarrow> ('n, 't) syms \<Rightarrow> 't rlexp" where
-  "rlexp_syms \<gamma>' w = rlexp_concats (map (rlexp_sym \<gamma>') w)"
-
-
-(* Some auxiliary lemmas *)
-
-lemma subst_lang_mono: "mono (subst_lang P)"
-  using mono_if_omega_cont[OF omega_cont_Lang_lfp] by blast
-
-lemma CFL_Lang_not_in_Prods_aux:
-  assumes "A \<notin> Nts P"
-    shows "((subst_lang P)^^n) (\<lambda>A. {}) A = {}"
-proof (cases n)
-  case (Suc nat)
-  from assms have "Rhss P A = {}" unfolding Nts_def Rhss_def by blast
-  with Suc show ?thesis unfolding subst_lang_def by simp
-qed auto
-
-lemma CFL_Lang_not_in_Prods: "A \<notin> Nts P \<Longrightarrow> Lang_lfp P A = {}"
-  by (simp add: Lang_lfp_eq_Lang Lang_empty_if_notin_Lhss Nts_Lhss_Rhs_Nts)
-
-
 locale CFG_eq_sys =
   fixes P :: "('n,'a) Prods"
   fixes S :: 'n
@@ -206,15 +155,25 @@ locale CFG_eq_sys =
   assumes bij_\<gamma>_\<gamma>':  "bij_Nt_Var (Nts P) \<gamma> \<gamma>'"
 begin
 
-abbreviation "CFG_sys sys \<equiv>
-  length sys = card (Nts P) \<and>
-    (\<forall>i < card (Nts P). reg_eval (sys ! i) \<and> (\<forall>x \<in> vars (sys ! i). x < card (Nts P))
-                        \<and> (\<forall>s L. (\<forall>A \<in> Nts P. s (\<gamma>' A) = L A)
-                            \<longrightarrow> eval (sys ! i) s = subst_lang P L (\<gamma> i)))"
+text \<open>The following definitions construct a regular language expression for a single production. This
+happens step by step, i.e. starting with a single symbol (terminal or non-terminal) and then extending
+this to a single production. The definitions closely follow the definitions \<^term>\<open>inst_sym\<close>,
+\<^term>\<open>concats\<close> and \<^term>\<open>inst_syms\<close> in \<^theory>\<open>CFG.CFL\<close>\<close>
 
-abbreviation "sol \<equiv> \<lambda>i. if i < card (Nts P) then Lang_lfp P (\<gamma> i) else {}"
+definition rlexp_sym :: "('n, 'a) sym \<Rightarrow> 'a rlexp" where
+  "rlexp_sym s = (case s of Tm a \<Rightarrow> Const {[a]} | Nt A \<Rightarrow> Var (\<gamma>' A))"
 
-lemma rlexp_sym_reg: "reg_eval (rlexp_sym \<gamma>' s)"
+definition rlexp_concats :: "'a rlexp list \<Rightarrow> 'a rlexp" where
+  "rlexp_concats fs = foldr Concat fs (Const {[]})"
+
+definition rlexp_syms :: "('n, 'a) syms \<Rightarrow> 'a rlexp" where
+  "rlexp_syms w = rlexp_concats (map rlexp_sym w)"
+
+
+text \<open>Now it is shown that the regular language expression constructed for a single production
+is \<^const>\<open>reg_eval\<close>. Again, this happens step by step:\<close>
+
+lemma rlexp_sym_reg: "reg_eval (rlexp_sym s)"
 unfolding rlexp_sym_def proof (induction s)
   case (Tm x)
   have "regular_lang {[x]}" by (meson lang.simps(3))
@@ -226,47 +185,53 @@ lemma rlexp_concats_reg:
     shows "reg_eval (rlexp_concats fs)"
   using assms epsilon_regular unfolding rlexp_concats_def by (induction fs) auto
 
-lemma rlexp_syms_reg: "reg_eval (rlexp_syms \<gamma>' w)"
+lemma rlexp_syms_reg: "reg_eval (rlexp_syms w)"
 proof -
-  from rlexp_sym_reg have "\<forall>s \<in> set w. reg_eval (rlexp_sym \<gamma>' s)" by blast
+  from rlexp_sym_reg have "\<forall>s \<in> set w. reg_eval (rlexp_sym s)" by blast
   with rlexp_concats_reg show ?thesis unfolding rlexp_syms_def
     by (metis (no_types, lifting) image_iff list.set_map)
 qed
 
 
+text \<open>The subsequent lemmas prove that all variables appearing in the regular language
+expression of a single production correspond to non-terminals appearing in the production:\<close>
+
 lemma rlexp_sym_vars_Nt:
   assumes "s (\<gamma>' A) = L A"
-    shows "vars (rlexp_sym \<gamma>' (Nt A)) = {\<gamma>' A}"
+    shows "vars (rlexp_sym (Nt A)) = {\<gamma>' A}"
   using assms unfolding rlexp_sym_def by simp
 
-lemma rlexp_sym_vars_Tm: "vars (rlexp_sym \<gamma>' (Tm x)) = {}"
+lemma rlexp_sym_vars_Tm: "vars (rlexp_sym (Tm x)) = {}"
   unfolding rlexp_sym_def by simp
 
 lemma rlexp_concats_vars: "vars (rlexp_concats fs) = \<Union>(vars ` set fs)"
   unfolding rlexp_concats_def by (induction fs) simp_all
 
 (* it even holds equality, but we will not need it *)
-lemma insts'_vars: "vars (rlexp_syms \<gamma>' w) \<subseteq> \<gamma>' ` nts_syms w"
+lemma insts'_vars: "vars (rlexp_syms w) \<subseteq> \<gamma>' ` nts_syms w"
 proof
   fix x
-  assume "x \<in> vars (rlexp_syms \<gamma>' w)"
-  with rlexp_concats_vars have "x \<in> \<Union>(vars ` set (map (rlexp_sym \<gamma>') w))"
+  assume "x \<in> vars (rlexp_syms w)"
+  with rlexp_concats_vars have "x \<in> \<Union>(vars ` set (map rlexp_sym w))"
     unfolding rlexp_syms_def by blast
-  then obtain f where *: "f \<in> set (map (rlexp_sym \<gamma>') w) \<and> x \<in> vars f" by blast
-  then obtain s where **: "s \<in> set w \<and> rlexp_sym \<gamma>' s = f" by auto
+  then obtain f where *: "f \<in> set (map rlexp_sym w) \<and> x \<in> vars f" by blast
+  then obtain s where **: "s \<in> set w \<and> rlexp_sym s = f" by auto
   with * rlexp_sym_vars_Tm obtain A where ***: "s = Nt A" by (metis empty_iff sym.exhaust)
   with ** have ****: "A \<in> nts_syms w" unfolding nts_syms_def by blast
-  with rlexp_sym_vars_Nt have "vars (rlexp_sym \<gamma>' (Nt A)) = {\<gamma>' A}" by blast
+  with rlexp_sym_vars_Nt have "vars (rlexp_sym (Nt A)) = {\<gamma>' A}" by blast
   with * ** *** **** show "x \<in> \<gamma>' ` nts_syms w" by blast
 qed
 
 
+text \<open>Evaluating the regular language expression of a single production under some valuation
+corresponds to instantiating the production according to the valuation:\<close>
+
 lemma rlexp_sym_inst_Nt:
   assumes "v (\<gamma>' A) = L A"
-    shows "eval (rlexp_sym \<gamma>' (Nt A)) v = inst_sym L (Nt A)"
+    shows "eval (rlexp_sym (Nt A)) v = inst_sym L (Nt A)"
   using assms unfolding rlexp_sym_def inst_sym_def by force
 
-lemma rlexp_sym_inst_Tm: "eval (rlexp_sym \<gamma>' (Tm a)) v = inst_sym L (Tm a)"
+lemma rlexp_sym_inst_Tm: "eval (rlexp_sym (Tm a)) v = inst_sym L (Tm a)"
   unfolding rlexp_sym_def inst_sym_def by force
 
 lemma rlexp_concats_concats:
@@ -286,13 +251,13 @@ qed
 
 lemma rlexp_syms_insts:
   assumes "\<forall>A \<in> nts_syms w. v (\<gamma>' A) = L A"
-    shows "eval (rlexp_syms \<gamma>' w) v = inst_syms L w"
+    shows "eval (rlexp_syms w) v = inst_syms L w"
 proof -
-  have "\<forall>i < length w. eval (rlexp_sym \<gamma>' (w!i)) v = inst_sym L (w!i)"
+  have "\<forall>i < length w. eval (rlexp_sym (w!i)) v = inst_sym L (w!i)"
   proof (rule allI, rule impI)
     fix i
     assume "i < length w"
-    then show "eval (rlexp_sym \<gamma>' (w ! i)) v = inst_sym L (w ! i)"
+    then show "eval (rlexp_sym (w ! i)) v = inst_sym L (w ! i)"
       using assms proof (induction "w!i")
       case (Nt A)
       then have "v (\<gamma>' A) = L A" unfolding nts_syms_def by force
@@ -307,11 +272,13 @@ proof -
 qed
 
 
+text \<open>Each non-terminal of the CFG induces some \<^const>\<open>reg_eval\<close> equation. We do not directly construct
+the equation but only prove its existence:\<close>
 lemma subst_lang_rlexp:
   "\<exists>eq. reg_eval eq \<and> vars eq \<subseteq> \<gamma>' ` Nts P
          \<and> (\<forall>v L. (\<forall>A \<in> Nts P. v (\<gamma>' A) = L A) \<longrightarrow> eval eq v = subst_lang P L A)"
 proof -
-  let ?Insts = "(rlexp_syms \<gamma>') ` (Rhss P A)"
+  let ?Insts = "rlexp_syms ` (Rhss P A)"
   from finite_Rhss[OF finite_P] have "finite ?Insts" by simp
   moreover from rlexp_syms_reg have "\<forall>f \<in> ?Insts. reg_eval f" by blast
   ultimately obtain eq where *: "reg_eval eq \<and> \<Union>(vars ` ?Insts) = vars eq
@@ -323,7 +290,7 @@ proof -
     fix x
     assume "x \<in> vars eq"
     with * obtain f where **: "f \<in> ?Insts \<and> x \<in> vars f" by blast
-    then obtain w where ***: "w \<in> Rhss P A \<and> f = rlexp_syms \<gamma>' w" by blast
+    then obtain w where ***: "w \<in> Rhss P A \<and> f = rlexp_syms w" by blast
     with ** insts'_vars have "x \<in> \<gamma>' ` nts_syms w" by auto
     with *** show "x \<in> \<gamma>' ` Nts P" unfolding Nts_def Rhss_def by blast
   qed
@@ -333,12 +300,12 @@ proof -
     fix v :: "nat \<Rightarrow> 'a lang" and L :: "'n \<Rightarrow> 'a lang"
     assume state_L: "\<forall>A \<in> Nts P. v (\<gamma>' A) = L A"
 
-    have "\<forall>w \<in> Rhss P A. eval (rlexp_syms \<gamma>' w) v = inst_syms L w"
+    have "\<forall>w \<in> Rhss P A. eval (rlexp_syms w) v = inst_syms L w"
     proof
       fix w
       assume "w \<in> Rhss P A"
       with state_L Nts_nts_syms have "\<forall>A \<in> nts_syms w. v (\<gamma>' A) = L A" by fast
-      from rlexp_syms_insts[OF this] show "eval (rlexp_syms \<gamma>' w) v = inst_syms L w" by blast
+      from rlexp_syms_insts[OF this] show "eval (rlexp_syms w) v = inst_syms L w" by blast
     qed
 
     then have "subst_lang P L A = (\<Union>f \<in> ?Insts. eval f v)" unfolding subst_lang_def by auto
@@ -348,6 +315,15 @@ proof -
   ultimately show ?thesis by auto
 qed
 
+
+text \<open>The whole CFG induces a system of equations. We first define which conditions this system
+should fulfill and show its existence in the second step:\<close>
+
+abbreviation "CFG_sys sys \<equiv>
+  length sys = card (Nts P) \<and>
+    (\<forall>i < card (Nts P). reg_eval (sys ! i) \<and> (\<forall>x \<in> vars (sys ! i). x < card (Nts P))
+                        \<and> (\<forall>s L. (\<forall>A \<in> Nts P. s (\<gamma>' A) = L A)
+                            \<longrightarrow> eval (sys ! i) s = subst_lang P L (\<gamma> i)))"
 
 lemma CFG_as_eq_sys: "\<exists>sys. CFG_sys sys"
 proof -
@@ -364,6 +340,13 @@ proof -
     show ?thesis by blast
 qed
 
+
+text \<open>As we have proved that each CFG induces a system of equations it remains to show that the
+ CFG's language is a minimal solution of this system. The first lemma proves that the CFG's language
+is a solution and the next two lemmas prove that it is minimal:\<close>
+
+abbreviation "sol \<equiv> \<lambda>i. if i < card (Nts P) then Lang_lfp P (\<gamma> i) else {}"
+
 lemma CFG_sys_CFL_is_sol:
   assumes "CFG_sys sys"
   shows "solves_ineq_sys sys sol"
@@ -375,7 +358,7 @@ unfolding solves_ineq_sys_def proof (rule allI, rule impI)
     unfolding bij_Nt_Var_def bij_betw_def by force
   with \<open>i < card (Nts P)\<close> assms have "eval (sys ! i) sol = subst_lang P (Lang_lfp P) (\<gamma> i)"
     by presburger
-  with lfp_fixpoint[OF subst_lang_mono] have 1: "eval (sys ! i) sol = Lang_lfp P (\<gamma> i)"
+  with lfp_fixpoint[OF mono_if_omega_cont[OF omega_cont_Lang_lfp]] have 1: "eval (sys ! i) sol = Lang_lfp P (\<gamma> i)"
     unfolding Lang_lfp_def by metis
 
   from \<open>i < card (Nts P)\<close> bij_\<gamma>_\<gamma>' have "\<gamma> i \<in> Nts P"
@@ -423,6 +406,10 @@ next
   then show ?thesis by auto
 qed
 
+
+text \<open>Lastly we combine all of the previous lemmas into the desired result of this section, namely
+that each CFG induces a system of equations such that the CFG's language is a minimal solution of
+the system:\<close>
 lemma CFL_is_min_sol:
   "\<exists>sys. (\<forall>eq \<in> set sys. reg_eval eq) \<and> (\<forall>eq \<in> set sys. \<forall>x \<in> vars eq. x < length sys)
           \<and> min_sol_ineq_sys sys sol"
@@ -440,10 +427,12 @@ qed
 end
 
 
-section \<open>Relationship between the system of equations with and the one without Parikh images\<close>
+subsection \<open>Relationship between the two types of systems of equations\<close>
 
-text \<open>To any solution \<open>sol\<close> of a commutative system of equations, there corresponds
-a solution to the same non-commutative system which has the same Parikh image as \<open>sol\<close>\<close>
+text \<open>One can simply convert a system \<open>sys\<close> of equations of the second type (i.e. the one with Parikh images)
+into a system of equations of the first type by dropping the Parikh images on both side of each equation.
+To any solution \<open>sol\<close> of \<open>sys\<close> then exists a valuation whose Parikh image is identical to that of
+\<open>sol\<close> and which is a solution of the other system (i.e. the system obtained by dropping all Parikh images in \<open>sys\<close>):\<close>
 lemma sol_comm_sol:
   assumes sol_is_sol_comm: "solves_ineq_sys_comm sys sol"
   shows   "\<exists>sol'. (\<forall>x. parikh_img (sol x) = parikh_img (sol' x)) \<and> solves_ineq_sys sys sol'"
@@ -469,8 +458,9 @@ proof
     by simp
 qed
 
-text \<open>A minimal solution of the non-commutative system of equations is a solution of the
-commutative system of equations, as well.\<close>
+text \<open>The converse works similarly: Given a minimal solution \<open>sol\<close> of the system \<open>sys\<close> of the first type,
+then \<open>sol\<close> is also a minimal solution to the system obtained by converting \<open>sys\<close> into a system of the second
+type (which can be achieved by applying the Parikh image on both sides of each equation):\<close>
 lemma min_sol_min_sol_comm:
   assumes "min_sol_ineq_sys sys sol"
     shows "min_sol_ineq_sys_comm sys sol"
@@ -491,7 +481,7 @@ unfolding min_sol_ineq_sys_comm_def proof
   qed
 qed
 
-text \<open>All minimal solutions of a commutative system of equations have the same Parikh image\<close>
+text \<open>All minimal solutions of a system of the second type have the same Parikh image:\<close>
 lemma min_sol_comm_unique:
   assumes sol1_is_min_sol: "min_sol_ineq_sys_comm sys sol1"
       and sol2_is_min_sol: "min_sol_ineq_sys_comm sys sol2"
